finish refactoring of Core

theories/Core/ContractEquations.v
@@ -1,18 +1,9 @@
-Require Import CSL.Contract2.  
-Require Import CSL.Order.
-Require Import Lists.List.
-Require Import Sorting.Permutation.
-Require Import Sorting.Mergesort.
-Require Import Sorting.Sorted.
-Require Import Bool.Bool.
-Require Import Bool.Sumbool.
-Require Import List Setoid Permutation Sorted Orders.
-Require Import Coq.Arith.PeanoNat.
+Require Import CSL.Core.Contract.  
+Require Import Lists.List Bool.Bool Bool.Sumbool Setoid Coq.Arith.PeanoNat.
+
 Import ListNotations.
 
 Set Implicit Arguments.
-
-Module Import TraceSort := Sort TraceOrder.
 
 Reserved Notation "c0 =R= c1" (at level 63).
 
@@ -244,10 +235,12 @@ intros. rewrite (c_eq_incl_plus_fold_aux H).
 rewrite (c_eq_incl_plus_fold_aux H0). apply c_eq_plus_fold_comm_app.
 Qed.
 
-Lemma comp_equiv_destruct : forall (c0 c1: Contract),(forall s : Trace, s =~ c0 <-> s =~ c1) ->
+Lemma comp_equiv_destruct : forall (c0 c1: Contract),(forall s : Trace, s =~ c0 <-> s =~ c1) <->
 (forall s : Trace, s =~ c0 -> s =~ c1) /\ (forall s : Trace, s =~ c1 -> s =~ c0).
 Proof.
-intros. split ; intros; specialize H with s; destruct H; auto.
+ split ; intros.
+- split;intros; specialize H with s; destruct H; auto.
+- destruct H. split;intros;auto.
 Qed.
 
 Lemma Matches_member : forall (s : Trace)(c : Contract), s =~ c -> In s (monoms c). 
@@ -267,11 +260,37 @@ split.
 - unfold contract_of_monom. apply seq_fold_map.
 Qed.
 
+Theorem Matches_iff_member : forall s c, s =~ c <-> In s (monoms c).
+Proof.
+split; auto using Matches_member,member_Matches.
+Qed.
+
 Lemma Matches_incl : forall (c0 c1 : Contract), (forall (s : Trace), s =~ c0 -> s =~ c1) -> 
 incl (monoms c0) (monoms c1).
 Proof.
 intros. unfold incl. intros. auto using Matches_member, member_Matches.
 Qed.
+
+Lemma incl_Matches : forall (c0 c1 : Contract), incl (monoms c0) (monoms c1) -> 
+(forall (s : Trace), s =~ c0 -> s =~ c1).
+Proof.
+intros. unfold incl in H. rewrite Matches_iff_member in *. auto.
+Qed.
+
+Theorem Matches_iff_incl : forall (c0 c1 : Contract), (forall (s : Trace), s =~ c0 -> s =~ c1) <-> 
+incl (monoms c0) (monoms c1).
+Proof.
+split;eauto using Matches_incl,incl_Matches.
+Qed.
+
+Corollary Matches_eq_iff_incl_and : forall (c0 c1 : Contract), (forall (s : Trace), s =~ c0 <-> s =~ c1) <-> 
+incl (monoms c0) (monoms c1) /\ incl (monoms c1) (monoms c0) .
+Proof.
+split;intros.
+- repeat rewrite <- Matches_iff_incl. now apply comp_equiv_destruct in H.
+- generalize s. rewrite comp_equiv_destruct. now repeat setoid_rewrite Matches_iff_incl.
+Qed.
+
 
 Lemma c_eq_completeness : forall (c0 c1 : Contract), (forall s : Trace, s =~ c0 <-> s =~ c1) -> c0 =R= c1.
 Proof.
@@ -281,187 +300,10 @@ apply Matches_incl in H0. apply Matches_incl in H1.
 apply c_eq_incl_plus_fold; apply incl_map;auto.
 Qed.
 
-
-(**********Solver***********)
-
-Inductive Expr :=
-| Var : nat -> Expr
-| ESuccess : Expr
-| EFailure : Expr
-| EPlus : Expr -> Expr -> Expr
-| ESeq : Expr -> Expr -> Expr.
-
-
-Fixpoint contract_of_Expr vals e :=
-match e with
-| Var v => vals v
-| ESuccess => Success
-| EFailure => Failure
-| EPlus e0 e1 => (contract_of_Expr vals e0) _+_ (contract_of_Expr vals e1)
-| ESeq e0 e1 => (contract_of_Expr vals e0) _;_ (contract_of_Expr vals e1)
-end.
-
-Fixpoint vars_lists_of_Expr (e : Expr) : list (list nat) :=
-match e with
-| Var v => [[v]]
-| ESuccess => [[]]
-| EFailure => []
-| EPlus e0 e1 => (vars_lists_of_Expr e0) ++ (vars_lists_of_Expr e1)
-| ESeq e0 e1 => map (fun (a : list nat * list nat) => let (a1,a2):=a in a1++a2) (list_prod (vars_lists_of_Expr e0) (vars_lists_of_Expr e1))
-end.
-
-
-Definition list_contract_of_Expr_vars (vals : nat -> Contract) (l : list (list nat)) := 
- map (fun l0 => seq_fold (map vals l0)) l.
-
-
-Check forallb.
-Check Nat.eq_dec.
-Locate nat_dec.
-
-Definition inclb (l0 l1 : list (list nat)) :bool := 
- forallb (fun a0 => existsb (fun a1 => if (list_eq_dec Nat.eq_dec) a0 a1 then true else false) l1) l0.
-
-Lemma inclb_iff : forall (l0 l1 : list (list nat)), inclb l0 l1 = true <-> incl l0 l1.
-Proof. unfold inclb. unfold incl. split. 
-- intros. rewrite forallb_forall in H. apply H in H0. rewrite existsb_exists in H0. destruct H0 as [x [P0 P1]].
-destruct (list_eq_dec Nat.eq_dec a x);subst;auto.
-discriminate.
-- intros. rewrite forallb_forall. intros. apply H in H0. rewrite existsb_exists. exists x. split;auto.
-  destruct (list_eq_dec Nat.eq_dec x x);auto.
-Qed.
-
-Lemma incl_reflect : forall (l0 l1 : list (list nat)), reflect (incl l0 l1) (inclb l0 l1).
-Proof. 
-intros. destruct (inclb l0 l1) eqn:Heqn.
-- constructor. now rewrite inclb_iff in Heqn.
-- constructor. intro H. rewrite <- inclb_iff in H. rewrite Heqn in H. discriminate.
-Qed.
-
-Definition expr_eqb (e0 e1 : Expr) := inclb (vars_lists_of_Expr e0) (vars_lists_of_Expr e1) && inclb (vars_lists_of_Expr e1) (vars_lists_of_Expr e0).
-
-Definition expr_eq e0 e1 := incl (vars_lists_of_Expr e0) (vars_lists_of_Expr e1) /\ incl (vars_lists_of_Expr e1) (vars_lists_of_Expr e0).
-
-Lemma expr_eq_reflect : forall (e0 e1 : Expr), reflect (expr_eq e0 e1) (expr_eqb e0 e1).
+Theorem Matches_iff_c_eq : forall c0 c1, (forall s, s =~ c0 <-> s =~ c1) <-> c0 =R= c1.
 Proof.
-intros. destruct (expr_eqb e0 e1) eqn:Heqn; unfold expr_eq; unfold expr_eqb in Heqn;
-constructor;repeat rewrite <- inclb_iff; auto using andb_prop.
-intro H. rewrite <- andb_true_iff in H.  rewrite H in Heqn. discriminate. 
+split; auto using c_eq_completeness, c_eq_soundness.
 Qed.
-
-
-Lemma expr_monoms : forall (e : Expr)(vals : nat -> Contract), contract_of_Expr vals e =R= plus_fold (map (fun l => seq_fold (map vals l)) (vars_lists_of_Expr e)).
-Proof.
-induction e;intros;simpl; try solve [auto_rwd_eqDB].
-- rewrite map_app. rewrite c_eq_plus_fold_app.
-  apply c_plus_morph;auto.
-- rewrite map_map. apply c_eq_completeness. intros. rewrite in_plus_fold. split;intros.
-  * inversion H. subst.
- 
-    eapply c_eq_soundness in IHe1.
-    rewrite in_plus_fold in IHe1. 
-    eapply IHe1 in H3. 
- 
-    eapply c_eq_soundness in IHe2. 
-    rewrite in_plus_fold in IHe2. 
-    eapply IHe2 in H4.
-
-    clear IHe1. clear IHe2.
-
-    destruct_ctx. rewrite in_map_iff in *. destruct_ctx.
-    exists (seq_fold (map vals (x2++x1))). 
-    rewrite map_app at 2. rewrite seq_fold_app. subst. 
-    split; try constructor; auto with eqDB.
-
-    rewrite in_map_iff. exists (x2,x1). split;auto.
-    rewrite in_prod_iff. split;auto.
-
-  * destruct_ctx. rewrite in_map_iff in H.
-    destruct_ctx. destruct x0. rewrite map_app in H.
-    specialize IHe1 with vals. specialize IHe2 with vals. 
-    pose proof (c_seq_morph IHe1 IHe2). apply c_eq_soundness with (s:=s) in H2.
-    rewrite H2. subst. rewrite seq_fold_app in H0. c_inversion.
-    constructor; rewrite in_plus_fold;
-    rewrite in_prod_iff in H1;destruct_ctx.
-    ** exists (seq_fold (map vals l));split;auto.
-       rewrite in_map_iff. exists l. split;auto.
-    ** exists (seq_fold (map vals l0));split;auto.
-       rewrite in_map_iff. exists l0. split;auto.
-Qed.
-
-Lemma c_eqP : forall (e0 e1 : Expr)(vals : nat -> Contract), expr_eqb e0 e1 = true -> (contract_of_Expr vals e0) =R= (contract_of_Expr vals e1).
-Proof.
-intros. repeat rewrite expr_monoms. apply c_eq_completeness. intros. repeat rewrite in_plus_fold. 
-destruct (expr_eq_reflect e0 e1);try discriminate.
-unfold expr_eq in e. split;intros;destruct_ctx;rewrite in_map_iff in H0;
-destruct_ctx;exists x; split;auto; rewrite in_map_iff; exists x0; split ; auto.
-Qed.
-
-Ltac intern vars e :=
-  let rec loop n vars' :=
-    match vars' with
-    | [] =>
-      let vars'' := eval simpl in (rev (e::(rev vars))) in
-      constr:((n, vars''))
-    | e :: ?vars'' => constr:((n, vars))
-    | _ :: ?vars'' => loop (S n) vars''
-    end in
-  loop 0 vars.
-
-Ltac reify_expr vars c :=
-  match c with
-  | ?c1 _+_ ?c2 =>
-    let r1 := reify_expr vars c1 in
-    match r1 with
-    | (?qe1, ?vars') =>
-      let r2 := reify_expr vars' c2 in
-      match r2 with
-      | (?qe2, ?vars'') => constr:((EPlus qe1 qe2, vars''))
-      end
-    end
-  | ?c1 _;_ ?c2 =>
-    let r1 := reify_expr vars c1 in
-    match r1 with
-    | (?qe1, ?vars') =>
-      let r2 := reify_expr vars' c2 in
-      match r2 with
-      | (?qe2, ?vars'') => constr:((ESeq qe1 qe2, vars''))
-      end
-    end
-  | _ =>
-    let r := intern vars c in
-    match r with
-    | (?n, ?vars') => constr:((Var n, vars'))
-    end
-  end.
-
-Fixpoint fun_of_list_aux (l : list  (nat * Contract)) :=
-match l with
-| [] => (fun  _ => Failure)
-| (n,c)::l' => let f2 := fun_of_list_aux l'
-               in (fun t => if Nat.eq_dec n t then c else f2 t)
-end.
-
-Definition fun_of_list l := fun_of_list_aux (combine (seq 0 (length l)) l).
-
-Ltac csl_solve :=
-  match goal with
-  | |- ?c1 =R= ?c2 =>
-    let r1 := reify_expr (@nil Contract) c1 in
-    match r1 with
-    | (?qe1, ?vm') =>
-      let r2 := reify_expr vm' c2 in
-      match r2 with
-      | (?qe2, ?vm'') => exact (@c_eqP qe1 qe2 (fun_of_list vm'') eq_refl) 
-      end
-    end
-  end.
-
-
-Lemma test2 : forall c0 c0' c1 c1', (c0 _+_ c1) _;_ (c0' _+_ c1') =R= 
-                     c0 _;_ c0' _+_ c0 _;_ c1' _+_ c1 _;_ c0' _+_ c1 _;_ c1'. 
-Proof. intros. csl_solve. Qed.
-
 
 
 
